theories/clang/lang.v
@@ -1,10 +1,7 @@
 (** Language definition **)
 
-From iris.algebra Require Import gmap.
 From iris.base_logic Require Export gen_heap big_op.
-From iris.algebra Require Export gmap agree auth frac excl.
-From iris.base_logic.lib Require Export wsat fancy_updates namespaces.
-From iris.proofmode Require Export tactics.
+From iris.algebra Require Import gmap.
 From iris_os.lib Require Export smap prelude.
 From iris_os.clang Require Export memory types.
 
